\input{./templatenst/prefs/jkf21.tex}
\input{./templatenst/prefs/me.tex}

\documentclass[10pt,\jkfside,a4paper]{article}

\input{./templatenst/includes.tex}
\input{./templatenst/template.tex}

\fancyhead[RO,LE]{{\bfseries NST Maths, SV~8}\\05-01-2022\ 12:00, Video Link}

\usepackage{physics}

\begin{document}

\section*{Ordinary Differential Equations}

\begin{enumerate}
\setcounter{enumi}{2}

\item
\begin{enumerate}

\item
\begin{equation}
\begin{split}
\dv{y}{x} &= - \frac{x^3}{(y + 1)^2}\\
(y + 1)^2 \dv{y}{x} &= -x^3\\
\frac{1}{3}(y + 1)^3 &= -\frac{1}{4}x^4 + c\\
(y + 1)^3 &= c - \frac{3}{4}x^4\\
y &= -1 + \sqrt[3]{c - \frac{3}{4}x^4}\\
\end{split}
\end{equation}

\item 
\begin{equation}
\begin{split}
\dv{y}{x} &= \frac{4y}{x(y - 3)}\\
\frac{y - 3}{y}\dv{y}{x} &= \frac{4}{x}\\
(1 - \frac{3}{y})\dv{y}{x} &= \frac{4}{x}\\
y - 3\ln{y} &= 4\ln{x} + c\\
\end{split}
\end{equation}

\end{enumerate}

\item
\begin{enumerate}

\item
\begin{equation}
\begin{split}
\dv{y}{x} + 2xy &= 4x\\
\mu(x) &= e^{\int 2x dx}\\
\mu(x) &= e^{x^2}\\
e^{x^2}\dv{y}{x} + 2xe^{x^2}y &= 4xe^{x^2}\\
ye^{x^2} &= 2e^{x^2} + c\\
y &= 3 + ce^{-x^2}\\
\end{split}
\end{equation}

\item 
\begin{equation}
\begin{split}
\dv{y}{x} + (2 - 3x^2)x^{-3}y &= 1\\
\mu(x) &= e^{\int \frac{2}{x^3} - \frac{3}{x}dx}\\
\mu(x) &= e^{-\frac{1}{x^2} - 3\ln{x}}\\
\mu(x) &= x^{-3}e^{-\frac{1}{x^2}}\\
x^{-3}e^{-\frac{1}{x^2}}\dv{y}{x} + (2 - 3x^2)x^{-6}e^{-\frac{1}{x^2}}y &= x^{-3}e^{-\frac{1}{x^2}}\\
x^{-3}e^{-\frac{1}{x^2}}y &= \frac{1}{2}e^{-\frac{1}{x^2}} + c\\
y &= \frac{1}{2}x^3 + cx^3e^{\frac{1}{x^2}}\\
\end{split}
\end{equation}

\end{enumerate}

\item
\begin{equation}
\begin{split}
v &= (x + y + 1)\\
\dv{v}{x} &= \dv{y}{x} + 1\\
(x + y + 1)^2\dv{y}{x} + (x + y + 1)^2 + x^3 &= 0\\
(x + y + 1)^2(\dv{y}{x} + 1) + x^3 &= 0\\
v^2\dv{v}{x} + x^3 &= 0\\
\frac{1}{3}v^3 + \frac{1}{4}x^4 &= c\\
v^3 &= c - \frac{3}{4}x^4\\
(x + y + 1)^3 &= c - \frac{3}{4}x^4\\
x + y + 1 &= \sqrt[3]{c - \frac{3}{4}x^4}\\
y &= -x - 1 + \sqrt[3]{c - \frac{3}{4}x^4}\\
\end{split}
\end{equation}

\item
\begin{enumerate}

\item
\begin{equation}
\begin{split}
v &= y^{-4}\\
\dv{v}{x} &= -4y^{-5}\dv{y}{x}\\
-\frac{y^5}{4}\dv{v}{x} &= \dv{y}{x}\\
\dv{y}{x} - y &= xy^5\\
-\frac{y^5}{4}\dv{v}{x} - y &= xy^5\\
\dv{v}{x} + 4y^{-4} &= -4x\\
\dv{v}{x} + 4v &= -4x\\
\mu(x) &= e^{\int 4 dx}\\
\mu(x) &= e^{4x}\\
e^{4x}\dv{v}{x} + 4ve^{4x} &= -4xe^{4x}\\
ve^{4x} &= -xe^{4x} + \frac{1}{4}e^{4x} + c\\
v &= -x + \frac{1}{4} + ce^{-4x}\\
\frac{1}{y^4} &= -x + \frac{1}{4} + ce^{-4x}\\
y &= \sqrt[4]{\frac{1}{-x + \frac{1}{4} + ce^{-4x}}}
\end{split}
\end{equation}

\item
\begin{equation}
\begin{split}
v &= \frac{1}{y}\\
\dv{v}{x} &= -\frac{1}{y^2}\dv{y}{x}\\
-y^2\dv{v}{x} &= \dv{y}{x}\\
\dv{y}{x} + y &= y^2(\cos{x} - \sin{x})\\
-y^2\dv{v}{x} + y &= y^2(\cos{x} - \sin{x})\\
\dv{v}{x} - \frac{1}{y} &= \sin{x} - \cos{x}\\
\dv{v}{x} - v &= \sin{x} - \cos{x}\\
\mu(x) &= e^{\int-1dx}\\
\mu{x} &= e^{-x}\\
e^{-x}\dv{v}{x} - ve^{-x} &= \sin{x}e^{-x} - \cos{x}e^{-x}\\
ve^{-x} &= -\sin{x}e^{-x} + c\\
v &= -\sin{x} + ce^x\\
\frac{1}{y} &= -\sin{x} + ce^x\\
y &= \frac{1}{-\sin{x} + ce^x}\\
\end{split}
\end{equation}

\end{enumerate}

\item
\begin{equation}
\begin{split}
y &= vx\\
\dv{y}{x} &= v + x\dv{v}{x}\\
(y - x)\dv{y}{x} + (2x + 3y) &= 0\\
x(vx - x)\dv{v}{x} + v(xv - x) + 2x + 3vx &= 0\\
x(vx - x)\dv{v}{x} + v^2x + 2vx + 2x &= 0\\
x(v - 1)\dv{v}{x} + v^2 + 2v + 2 &= 0\\
x(v - 1)\dv{v}{x} &= -(v^2 + 2v + 2)\\
\frac{v - 1}{v^2 + 2v + 2}\dv{v}{x} &= -\frac{1}{x}\\
\left(\frac{v + 1}{v^2 + 2v + 2} - \frac{2}{(v + 1)^2 + 1}\right)\dv{v}{x} &= -\frac{1}{x}\\
\frac{1}{2}\ln(v^2 + 2v + 2) - 2\arctan(v + 1) &= -\ln Ax\\
\frac{1}{2}\ln(\frac{y^2}{x^2} + \frac{2y}{x} + 2) - 2\arctan{\left(\frac{y}{x} + 1\right)} &= - \ln Ax\\
\end{split}
\end{equation}

\item
\begin{enumerate}

\item
\begin{equation}
\begin{split}
v &= \frac{y}{x}\\
y &= vx\\
\dv{y}{x} &= v + x\dv{v}{x}\\
\dv{y}{x} &= \frac{y}{x} + \tan(\frac{y}{x})\\
v + x\dv{v}{x} &= v + \tan{v}\\
x\dv{v}{x} &= \tan{v}\\
\cot{v}\dv{v}{x} &= \frac{1}{x}\\
\ln{\sin{v}} &= \ln{Ax}\\
\sin{v} &= Ax\\
\sin{\frac{y}{x}} &= Ax\\
y &= x\arcsin{Ax}\\
\end{split}
\end{equation}

\item
\begin{equation}
\begin{split}
\ln y &= vx\\
\frac{1}{y}\dv{y}{x} &= v + x\dv{v}{x}\\
\dv{y}{x} &= y\left(v + x\dv{v}{x}\right)\\
(\ln y - x)\dv{y}{x} - y\ln y &= 0\\
y(\ln y - x)\left(v + x\dv{v}{x}\right) - y\ln y &= 0\\
y(xv - x)\left(v + x\dv{v}{x}\right) - yxv &= 0\\
(v - 1)\left(v + x\dv{v}{x}\right) - v &= 0\\
v^2 - v + x(v - 1)\dv{v}{x} - v &= 0\\
x(v - 1)\dv{v}{x} &= -(v^2 - 2v)\\
\frac{v - 1}{v(v - 2)}\dv{v}{x} &= -\frac{1}{x}\\
\left(\frac{1}{2v} - \frac{1}{2(v - 2)}\right)\dv{v}{x} &= -\frac{1}{x}\\
\frac{1}{2}\ln v + \frac{1}{2}\ln (v - 2) &= -\ln Ax\\
\ln v + \ln (v - 2) &= -2 \ln Ax\\
\ln (v(v - 2)) &= \ln \frac{1}{(Ax)^2}\\
v(v - 2) &= \frac{1}{(Ax)^2}\\
\ln y\left(\ln y - 2x^2\right) &= \frac{1}{C}\\
\end{split}
\end{equation}

\item
\begin{equation}
\begin{split}
v &= xy\\
y &= \frac{v}{x}\\
\dv{y}{x} &= -\frac{v}{x^2} + \frac{1}{x}\dv{v}{x}\\
\dv{y}{x} &= -\frac{y}{x} + \frac{1}{x}\dv{v}{x}\\
xy\dv{y}{x} + (x^2 + y^2 + x) &= 0\\
xy\left(-\frac{y}{x} + \frac{1}{x}\dv{v}{x}\right) + (x^2 + y^2 + x) &= 0\\
-y^2 + y\dv{v}{x} + x^2 + y^2 + x &= 0\\
\frac{v}{x}\dv{v}{x} + x^2 + x &= 0\\
v\dv{v}{x} + x^3 + x^2 &= 0\\
\frac{1}{2}v^2 + \frac{1}{4}x^4 + \frac{1}{3}x^3 &= c\\
x^2y^2 + \frac{1}{2}x^4 + \frac{2}{3}x^3 &= c\\
y^2 &= cx^{-2} - \frac{1}{2}x^2 - \frac{2}{3}x\\
y &= \sqrt{cx^{-2} - \frac{1}{2}x^2 - \frac{2}{3}x}\\
\end{split}
\end{equation}

\end{enumerate}

\end{enumerate}

\end{document}